Include additional lemmas that are needed for VSU_DrySafe.v

floyd/VSU.v
@@ -3270,6 +3270,495 @@ Proof.
   destruct g; auto.
   f_equal; auto.
 Qed.
+Check @Comp_prog_OK.
+
+Section WholeComp_semaxprogConstructive.
+Variable Espec : OracleKind.
+Variable Externs : funspecs.
+Variable p : QP.program function.
+Variable Exports : funspecs.
+Variable GP : globals -> mpred.
+Variable mainspec : funspec.
+Variable G: list(ident * funspec).
+Variable c: @Component Espec (QPvarspecs p) Externs nil p Exports GP (G_merge
+                 [(QP.prog_main p, mainspec)] G).
+
+Lemma WholeComponent_semax_progConstructive: forall
+  (NOMAIN: find_id (QP.prog_main p) G = None)
+  (z: OK_ty)
+  (MAIN: exists post, mainspec = QPmain_spec_ext' p z post)
+  (MAIN': isSome (PTree.get (QP.prog_main p) (QP.prog_defs p)))
+  (EXT_OK: all_unspecified_OK p)
+  (ALIGNED: QPall_initializers_aligned p = true) (* should be part of QPprogram_OK *)
+  (DEFS_NOT_BUILTIN: forallb not_builtin (PTree.elements (QP.prog_defs p)) = true)  (* should be part of QPprogram_OK *)
+  (CBC: forall H,
+    cenv_built_correctly
+        (map compdef_of_compenv_element
+           (sort_rank (PTree.elements (QP.prog_comp_env p)) []))
+         (composite_env_of_QPcomposite_env (QP.prog_comp_env p) H) 
+           = Errors.OK tt),
+let CBC1 := CBC _ in
+@semax_prog Espec (Comp_cs c)
+   (wholeprog_of_QPprog p (Comp_prog_OK c)
+    (cenv_built_correctly_e
+         (map compdef_of_compenv_element
+            (sort_rank (PTree.elements (QP.prog_comp_env p)) []))
+         (composite_env_of_QPcomposite_env (QP.prog_comp_env p) (projT1 (proj2 (Comp_prog_OK c))))
+         CBC1))
+    z (QPvarspecs p) 
+      (G_merge [(QP.prog_main p, mainspec)] G).
+Proof.
+  intros.
+ pose (prog := prog_of_component c (CBC _)).
+ split3; [ | | split3; [ | | split]].
+ 4: change SeparationLogicAsLogicSoundness.MainTheorem.CSHL_MinimumLogic.CSHL_Def.semax_func
+  with semax_func.
+-
+ subst prog; simpl.
+ unfold prog_defs_names. simpl.
+ apply compute_list_norepet_i.
+ clear - c.
+ rewrite map_app.
+ destruct (Comp_prog_OK c).
+ rewrite map_map. 
+ replace (fun x : ident * QP.builtin => fst (of_builtin x)) with (@fst ident QP.builtin); auto.
+ extensionality x. destruct x,b; simpl; auto.
+-
+ red. unfold SeparationLogic.prog_vars;
+ subst prog; simpl.
+ clear - ALIGNED.
+ unfold QPall_initializers_aligned in *.
+ unfold QPprog_vars in ALIGNED.
+  replace  (SeparationLogic.prog_vars'
+     (map of_builtin (QP.prog_builtins p) ++ PTree.elements (QP.prog_defs p)))
+    with  (SeparationLogic.prog_vars'(PTree.elements (QP.prog_defs p)))
+       by (induction (QP.prog_builtins p) as [|[i ?]]; try destruct b; simpl; auto).
+ induction (PTree.elements (QP.prog_defs p)) as [|[i?]]; auto.
+ destruct g; auto.
+ simpl in ALIGNED|-*.
+ rewrite andb_true_iff in ALIGNED|-*; destruct ALIGNED; auto.
+-
+  f_equal.
+  apply (proj1 (QPcompspecs_OK_e _ (proj2 (Comp_prog_OK c)))).
+-
+ apply (@WholeComponent_semax_func _ _ _ _ _ _ c EXT_OK DEFS_NOT_BUILTIN).
+-
+  subst prog; simpl.
+  unfold QPvarspecs, QPprog_vars, SeparationLogic.prog_vars. simpl.
+  clear.
+  replace  (SeparationLogic.prog_vars'
+     (map of_builtin (QP.prog_builtins p) ++ PTree.elements (QP.prog_defs p)))
+    with  (SeparationLogic.prog_vars'(PTree.elements (QP.prog_defs p)))
+       by (induction (QP.prog_builtins p) as [|[i ?]]; try destruct b; simpl; auto).
+  induction (PTree.elements (QP.prog_defs p)) as [|[i?]].
+  simpl. auto.
+  simpl. destruct g; auto.
+  simpl.
+  rewrite eqb_ident_true by auto.
+  rewrite eqb_type_refl by auto.
+  simpl; auto.
+- simpl find_id.
+   unfold augment_funspecs.
+   change SeparationLogic.prog_funct with prog_funct.
+   erewrite prog_funct_QP_prog_funct; [ | reflexivity].
+  set (G1 := G_merge [(QP.prog_main p, mainspec)] G).
+   destruct (augment_funspecs'_exists G1 (QP.prog_builtins p) (QPprog_funct p)) 
+     as [G' ?]; auto.
+   * 
+   apply (list_norepet_append_left _ _ (proj1 (Comp_prog_OK c))).
+   *
+   pose proof (list_norepet_append_right _ _ (proj1 (Comp_prog_OK c))).
+   unfold QPprog_funct.
+   clear - H. forget (PTree.elements (QP.prog_defs p)) as al.
+   induction al as [|[i[|]]]; simpl in *; auto. inv H; constructor; auto.
+   contradict H2. clear - H2; induction al as [|[j[|]]]; simpl in *; auto. destruct H2; auto.
+   inv H; auto.
+   *
+   assert (H1 := proj1 (Comp_prog_OK c)).
+   rewrite list_norepet_app in H1; destruct H1 as [_ [_ H1]].
+   eapply assoclists.list_disjoint_mono; try apply H1; auto.
+   clear; intros. unfold QPprog_funct in H.
+   induction (PTree.elements (QP.prog_defs p)) as [|[i[|]]]; simpl in *; auto. destruct H; auto.
+   *
+   clear - DEFS_NOT_BUILTIN.
+   unfold QPprog_funct. induction (PTree.elements (QP.prog_defs p)) as [|[i[|]]]; simpl in *; auto.
+   rewrite andb_true_iff in *|-*. tauto.
+   *
+     apply (Comp_G_LNR c).
+   *
+   intros.
+   fold G1 in c.
+   rewrite <- (Comp_G_dom c) in H.
+   rewrite in_app in H; destruct H.
+   apply IntIDs_elim in H; destruct H.
+   unfold QPprog_funct.
+   clear - H. induction (PTree.elements (QP.prog_defs p)) as [|[j[|]]]; simpl in *; auto.
+   destruct H; auto. inv H; auto.   destruct H; auto. inv H; auto.
+   apply (Comp_Externs c i) in H.
+   destruct H as [? [? [? [? ?]]]].
+   apply PTree.elements_correct in H.
+   unfold QPprog_funct.
+   clear - H. induction (PTree.elements (QP.prog_defs p)) as [|[j[|]]]; simpl in *; auto.
+   destruct H; auto. inv H; auto.   destruct H; auto. inv H; auto.
+   *
+   change (G_merge _ _) with G1.
+   rewrite H.
+   apply augment_funspecs'_e in H.
+   destruct MAIN as [post MAIN].
+   change (prog_main prog) with (QP.prog_main p).
+   assert   (MAINx: find_id (QP.prog_main p) G1 = Some (QPmain_spec_ext' p z post)). {
+     apply G_merge_find_id_SomeNone.
+     simpl. rewrite if_true by auto. f_equal; auto. auto.
+   }
+   rewrite (augment_funspecs_find_id_Some _ _ _ H (Comp_G_LNR c) _ _ MAINx).
+   exists post.
+   unfold QPmain_spec_ext', main_spec_ext'.
+   f_equal.
+   subst prog. unfold main_pre, SeparationLogic.main_pre.
+   unfold SeparationLogic.prog_vars. simpl.
+   unfold QPprog_vars.
+   replace  (SeparationLogic.prog_vars'
+     (map of_builtin (QP.prog_builtins p) ++ PTree.elements (QP.prog_defs p)))
+    with  (SeparationLogic.prog_vars'(PTree.elements (QP.prog_defs p)))
+       by (clear; induction (QP.prog_builtins p) as [|[i ?]]; try destruct b; simpl; auto).
+   extensionality gv rho.
+   normalize. f_equal. f_equal. f_equal. f_equal.
+  clear.
+  induction (PTree.elements (QP.prog_defs p)) as [|[i?]]; auto.
+  simpl.
+  destruct g; auto.
+  f_equal; auto.
+Qed.
+
+End WholeComp_semaxprogConstructive.
+
+(*another variant, currently unused*)
+Definition WholeProgSafeType' {Espec E p Exports GP mainspec} G
+       (c: find_id (QP.prog_main p) G = None /\
+             @Component Espec (QPvarspecs p) E nil p Exports GP 
+         (G_merge
+                 [(QP.prog_main p, mainspec)] G))
+             (z: @OK_ty Espec) :=
+ exists cs, exists OK, exists CBC, (*exists G, *)
+@semax_prog Espec cs
+   (wholeprog_of_QPprog p OK
+    (cenv_built_correctly_e
+         (map compdef_of_compenv_element
+            (sort_rank (PTree.elements (QP.prog_comp_env p)) []))
+         (composite_env_of_QPcomposite_env (QP.prog_comp_env p) (projT1 (proj2 OK)))
+         CBC))
+    z (QPvarspecs p) 
+      (G_merge [(QP.prog_main p, mainspec)] G).
+
+Lemma WholeComponent_semax_prog':
+ forall {Espec Externs p Exports GP mainspec} G
+  (c:  
+    find_id (QP.prog_main p) G = None /\
+     @Component Espec (QPvarspecs p) Externs nil p Exports GP (G_merge
+                 [(QP.prog_main p, mainspec)] G))
+  (NOMAIN:find_id (QP.prog_main p) G = None)
+  (z: OK_ty)
+  (MAIN: exists post, mainspec = QPmain_spec_ext' p z post)
+  (MAIN': isSome (PTree.get (QP.prog_main p) (QP.prog_defs p)))
+  (EXT_OK: all_unspecified_OK p)
+  (ALIGNED: QPall_initializers_aligned p = true) (* should be part of QPprogram_OK *)
+  (DEFS_NOT_BUILTIN: forallb not_builtin (PTree.elements (QP.prog_defs p)) = true)  (* should be part of QPprogram_OK *)
+  (CBC: forall H,
+    cenv_built_correctly
+        (map compdef_of_compenv_element
+           (sort_rank (PTree.elements (QP.prog_comp_env p)) []))
+         (composite_env_of_QPcomposite_env (QP.prog_comp_env p) H) 
+           = Errors.OK tt),
+  WholeProgSafeType' G c z.
+Proof.
+ intros ? ? ? ? ? mainspec; intros.
+ destruct c as [NO_MAIN c].
+ pose (prog := prog_of_component c (CBC _)).
+ red.
+ exists (Comp_cs c).
+ exists (Comp_prog_OK c).
+ exists (CBC _).
+(* exists G.*)
+ split3; [ | | split3; [ | | split]].
+ 4: change SeparationLogicAsLogicSoundness.MainTheorem.CSHL_MinimumLogic.CSHL_Def.semax_func
+  with semax_func.
+-
+ subst prog; simpl.
+ unfold prog_defs_names. simpl.
+ apply compute_list_norepet_i.
+ clear - c.
+ rewrite map_app.
+ destruct (Comp_prog_OK c).
+ rewrite map_map. 
+ replace (fun x : ident * QP.builtin => fst (of_builtin x)) with (@fst ident QP.builtin); auto.
+ extensionality x. destruct x,b; simpl; auto.
+-
+ red. unfold SeparationLogic.prog_vars;
+ subst prog; simpl.
+ clear - ALIGNED.
+ unfold QPall_initializers_aligned in *.
+ unfold QPprog_vars in ALIGNED.
+  replace  (SeparationLogic.prog_vars'
+     (map of_builtin (QP.prog_builtins p) ++ PTree.elements (QP.prog_defs p)))
+    with  (SeparationLogic.prog_vars'(PTree.elements (QP.prog_defs p)))
+       by (induction (QP.prog_builtins p) as [|[i ?]]; try destruct b; simpl; auto).
+ induction (PTree.elements (QP.prog_defs p)) as [|[i?]]; auto.
+ destruct g; auto.
+ simpl in ALIGNED|-*.
+ rewrite andb_true_iff in ALIGNED|-*; destruct ALIGNED; auto.
+-
+  f_equal.
+  apply (proj1 (QPcompspecs_OK_e _ (proj2 (Comp_prog_OK c)))).
+-
+ apply (@WholeComponent_semax_func _ _ _ _ _ _ c EXT_OK DEFS_NOT_BUILTIN).
+-
+  subst prog; simpl.
+  unfold QPvarspecs, QPprog_vars, SeparationLogic.prog_vars. simpl.
+  clear.
+  replace  (SeparationLogic.prog_vars'
+     (map of_builtin (QP.prog_builtins p) ++ PTree.elements (QP.prog_defs p)))
+    with  (SeparationLogic.prog_vars'(PTree.elements (QP.prog_defs p)))
+       by (induction (QP.prog_builtins p) as [|[i ?]]; try destruct b; simpl; auto).
+  induction (PTree.elements (QP.prog_defs p)) as [|[i?]].
+  simpl. auto.
+  simpl. destruct g; auto.
+  simpl.
+  rewrite eqb_ident_true by auto.
+  rewrite eqb_type_refl by auto.
+  simpl; auto.
+- simpl find_id.
+   unfold augment_funspecs.
+   change SeparationLogic.prog_funct with prog_funct.
+   erewrite prog_funct_QP_prog_funct; [ | reflexivity].
+  set (G1 := G_merge [(QP.prog_main p, mainspec)] G).
+   destruct (augment_funspecs'_exists G1 (QP.prog_builtins p) (QPprog_funct p)) 
+     as [G' ?]; auto.
+   * 
+   apply (list_norepet_append_left _ _ (proj1 (Comp_prog_OK c))).
+   *
+   pose proof (list_norepet_append_right _ _ (proj1 (Comp_prog_OK c))).
+   unfold QPprog_funct.
+   clear - H. forget (PTree.elements (QP.prog_defs p)) as al.
+   induction al as [|[i[|]]]; simpl in *; auto. inv H; constructor; auto.
+   contradict H2. clear - H2; induction al as [|[j[|]]]; simpl in *; auto. destruct H2; auto.
+   inv H; auto.
+   *
+   assert (H1 := proj1 (Comp_prog_OK c)).
+   rewrite list_norepet_app in H1; destruct H1 as [_ [_ H1]].
+   eapply assoclists.list_disjoint_mono; try apply H1; auto.
+   clear; intros. unfold QPprog_funct in H.
+   induction (PTree.elements (QP.prog_defs p)) as [|[i[|]]]; simpl in *; auto. destruct H; auto.
+   *
+   clear - DEFS_NOT_BUILTIN.
+   unfold QPprog_funct. induction (PTree.elements (QP.prog_defs p)) as [|[i[|]]]; simpl in *; auto.
+   rewrite andb_true_iff in *|-*. tauto.
+   *
+     apply (Comp_G_LNR c).
+   *
+   intros.
+   fold G1 in c.
+   rewrite <- (Comp_G_dom c) in H.
+   rewrite in_app in H; destruct H.
+   apply IntIDs_elim in H; destruct H.
+   unfold QPprog_funct.
+   clear - H. induction (PTree.elements (QP.prog_defs p)) as [|[j[|]]]; simpl in *; auto.
+   destruct H; auto. inv H; auto.   destruct H; auto. inv H; auto.
+   apply (Comp_Externs c i) in H.
+   destruct H as [? [? [? [? ?]]]].
+   apply PTree.elements_correct in H.
+   unfold QPprog_funct.
+   clear - H. induction (PTree.elements (QP.prog_defs p)) as [|[j[|]]]; simpl in *; auto.
+   destruct H; auto. inv H; auto.   destruct H; auto. inv H; auto.
+   *
+   change (G_merge _ _) with G1.
+   rewrite H.
+   apply augment_funspecs'_e in H.
+   destruct MAIN as [post MAIN].
+   change (prog_main prog) with (QP.prog_main p).
+   assert   (MAINx: find_id (QP.prog_main p) G1 = Some (QPmain_spec_ext' p z post)). {
+     apply G_merge_find_id_SomeNone.
+     simpl. rewrite if_true by auto. f_equal; auto. auto.
+   }
+   rewrite (augment_funspecs_find_id_Some _ _ _ H (Comp_G_LNR c) _ _ MAINx).
+   exists post.
+   unfold QPmain_spec_ext', main_spec_ext'.
+   f_equal.
+   subst prog. unfold main_pre, SeparationLogic.main_pre.
+   unfold SeparationLogic.prog_vars. simpl.
+   unfold QPprog_vars.
+   replace  (SeparationLogic.prog_vars'
+     (map of_builtin (QP.prog_builtins p) ++ PTree.elements (QP.prog_defs p)))
+    with  (SeparationLogic.prog_vars'(PTree.elements (QP.prog_defs p)))
+       by (clear; induction (QP.prog_builtins p) as [|[i ?]]; try destruct b; simpl; auto).
+   extensionality gv rho.
+   normalize. f_equal. f_equal. f_equal. f_equal.
+  clear.
+  induction (PTree.elements (QP.prog_defs p)) as [|[i?]]; auto.
+  simpl.
+  destruct g; auto.
+  f_equal; auto.
+Qed.
+
+(*another variant, currently unused*)
+Definition WholeProgSafeType'' {Espec E p Exports GP mainspec} G
+       (NOMAIN:find_id (QP.prog_main p) G = None)
+        (COMP: @Component Espec (QPvarspecs p) E nil p Exports GP
+         (G_merge
+                 [(QP.prog_main p, mainspec)] G))
+             (z: @OK_ty Espec) :=
+ exists cs, (*exists OK, *)exists CBC, (*exists G, *)
+@semax_prog Espec cs (prog_of_component COMP CBC)
+    z (QPvarspecs p) 
+      (G_merge [(QP.prog_main p, mainspec)] G).
+
+Lemma WholeComponent_semax_prog'':
+ forall {Espec Externs p Exports GP mainspec} G
+  (NOMAIN:
+    find_id (QP.prog_main p) G = None )
+  (COMP: @Component Espec (QPvarspecs p) Externs nil p Exports GP (G_merge
+                 [(QP.prog_main p, mainspec)] G))
+  (z: OK_ty)
+  (MAIN: exists post, mainspec = QPmain_spec_ext' p z post)
+  (MAIN': isSome (PTree.get (QP.prog_main p) (QP.prog_defs p)))
+  (EXT_OK: all_unspecified_OK p)
+  (ALIGNED: QPall_initializers_aligned p = true) (* should be part of QPprogram_OK *)
+  (DEFS_NOT_BUILTIN: forallb not_builtin (PTree.elements (QP.prog_defs p)) = true)  (* should be part of QPprogram_OK *)
+  (CBC: forall H,
+    cenv_built_correctly
+        (map compdef_of_compenv_element
+           (sort_rank (PTree.elements (QP.prog_comp_env p)) []))
+         (composite_env_of_QPcomposite_env (QP.prog_comp_env p) H) 
+           = Errors.OK tt),
+  WholeProgSafeType'' G NOMAIN COMP z.
+Proof.
+ intros ? ? ? ? ? mainspec; intros.
+(* destruct c as [NO_MAIN c].
+ pose (prog := prog_of_component c (CBC _)).*)
+ red.
+ rename COMP into c.
+ exists (Comp_cs c).
+ (*exists (Comp_prog_OK c).*)
+ exists (CBC _).
+(* exists G.*)
+ split3; [ | | split3; [ | | split]].
+ 4: change SeparationLogicAsLogicSoundness.MainTheorem.CSHL_MinimumLogic.CSHL_Def.semax_func
+  with semax_func.
+-
+ (*subst prog;*) simpl.
+ unfold prog_defs_names. simpl.
+ apply compute_list_norepet_i.
+ clear - c.
+ rewrite map_app.
+ destruct (Comp_prog_OK c).
+ rewrite map_map. 
+ replace (fun x : ident * QP.builtin => fst (of_builtin x)) with (@fst ident QP.builtin); auto.
+ extensionality x. destruct x,b; simpl; auto.
+-
+ red. unfold SeparationLogic.prog_vars;
+ (*subst prog;*) simpl.
+ clear - ALIGNED.
+ unfold QPall_initializers_aligned in *.
+ unfold QPprog_vars in ALIGNED.
+  replace  (SeparationLogic.prog_vars'
+     (map of_builtin (QP.prog_builtins p) ++ PTree.elements (QP.prog_defs p)))
+    with  (SeparationLogic.prog_vars'(PTree.elements (QP.prog_defs p)))
+       by (induction (QP.prog_builtins p) as [|[i ?]]; try destruct b; simpl; auto).
+ induction (PTree.elements (QP.prog_defs p)) as [|[i?]]; auto.
+ destruct g; auto.
+ simpl in ALIGNED|-*.
+ rewrite andb_true_iff in ALIGNED|-*; destruct ALIGNED; auto.
+-
+  f_equal.
+  apply (proj1 (QPcompspecs_OK_e _ (proj2 (Comp_prog_OK c)))).
+-
+ apply (@WholeComponent_semax_func _ _ _ _ _ _ c EXT_OK DEFS_NOT_BUILTIN).
+-
+  (*subst prog;*) simpl.
+  unfold QPvarspecs, QPprog_vars, SeparationLogic.prog_vars. simpl.
+  clear.
+  replace  (SeparationLogic.prog_vars'
+     (map of_builtin (QP.prog_builtins p) ++ PTree.elements (QP.prog_defs p)))
+    with  (SeparationLogic.prog_vars'(PTree.elements (QP.prog_defs p)))
+       by (induction (QP.prog_builtins p) as [|[i ?]]; try destruct b; simpl; auto).
+  induction (PTree.elements (QP.prog_defs p)) as [|[i?]].
+  simpl. auto.
+  simpl. destruct g; auto.
+  simpl.
+  rewrite eqb_ident_true by auto.
+  rewrite eqb_type_refl by auto.
+  simpl; auto.
+- simpl find_id.
+   unfold augment_funspecs.
+   change SeparationLogic.prog_funct with prog_funct.
+   erewrite prog_funct_QP_prog_funct; [ | reflexivity].
+  set (G1 := G_merge [(QP.prog_main p, mainspec)] G).
+   destruct (augment_funspecs'_exists G1 (QP.prog_builtins p) (QPprog_funct p)) 
+     as [G' ?]; auto.
+   * 
+   apply (list_norepet_append_left _ _ (proj1 (Comp_prog_OK c))).
+   *
+   pose proof (list_norepet_append_right _ _ (proj1 (Comp_prog_OK c))).
+   unfold QPprog_funct.
+   clear - H. forget (PTree.elements (QP.prog_defs p)) as al.
+   induction al as [|[i[|]]]; simpl in *; auto. inv H; constructor; auto.
+   contradict H2. clear - H2; induction al as [|[j[|]]]; simpl in *; auto. destruct H2; auto.
+   inv H; auto.
+   *
+   assert (H1 := proj1 (Comp_prog_OK c)).
+   rewrite list_norepet_app in H1; destruct H1 as [_ [_ H1]].
+   eapply assoclists.list_disjoint_mono; try apply H1; auto.
+   clear; intros. unfold QPprog_funct in H.
+   induction (PTree.elements (QP.prog_defs p)) as [|[i[|]]]; simpl in *; auto. destruct H; auto.
+   *
+   clear - DEFS_NOT_BUILTIN.
+   unfold QPprog_funct. induction (PTree.elements (QP.prog_defs p)) as [|[i[|]]]; simpl in *; auto.
+   rewrite andb_true_iff in *|-*. tauto.
+   *
+     apply (Comp_G_LNR c).
+   *
+   intros.
+   fold G1 in c.
+   rewrite <- (Comp_G_dom c) in H.
+   rewrite in_app in H; destruct H.
+   apply IntIDs_elim in H; destruct H.
+   unfold QPprog_funct.
+   clear - H. induction (PTree.elements (QP.prog_defs p)) as [|[j[|]]]; simpl in *; auto.
+   destruct H; auto. inv H; auto.   destruct H; auto. inv H; auto.
+   apply (Comp_Externs c i) in H.
+   destruct H as [? [? [? [? ?]]]].
+   apply PTree.elements_correct in H.
+   unfold QPprog_funct.
+   clear - H. induction (PTree.elements (QP.prog_defs p)) as [|[j[|]]]; simpl in *; auto.
+   destruct H; auto. inv H; auto.   destruct H; auto. inv H; auto.
+   *
+   change (G_merge _ _) with G1.
+   rewrite H.
+   apply augment_funspecs'_e in H.
+   destruct MAIN as [post MAIN].
+   (*change (prog_main prog) with (QP.prog_main p).*)
+   assert   (MAINx: find_id (QP.prog_main p) G1 = Some (QPmain_spec_ext' p z post)). {
+     apply G_merge_find_id_SomeNone.
+     simpl. rewrite if_true by auto. f_equal; auto. auto.
+   }
+   rewrite (augment_funspecs_find_id_Some _ _ _ H (Comp_G_LNR c) _ _ MAINx).
+   exists post.
+   unfold QPmain_spec_ext', main_spec_ext'.
+   f_equal.
+   (*subst prog.*) unfold main_pre, SeparationLogic.main_pre.
+   unfold SeparationLogic.prog_vars. simpl.
+   unfold QPprog_vars.
+   replace  (SeparationLogic.prog_vars'
+     (map of_builtin (QP.prog_builtins p) ++ PTree.elements (QP.prog_defs p)))
+    with  (SeparationLogic.prog_vars'(PTree.elements (QP.prog_defs p)))
+       by (clear; induction (QP.prog_builtins p) as [|[i ?]]; try destruct b; simpl; auto).
+   extensionality gv rho.
+   normalize. f_equal. f_equal. f_equal. f_equal.
+  clear.
+  induction (PTree.elements (QP.prog_defs p)) as [|[i?]]; auto.
+  simpl.
+  destruct g; auto.
+  f_equal; auto.
+Qed.
 
 Ltac QPlink_prog_tac p1 p2 :=
   let p' :=  uconstr:(QPlink_progs p1 p2) in
